Fix clean spec for get_attr in ConcurrentFS
Re-write FS invariant in terms of separation logic, exposing much more
in parameters to the rep function based on what is needed to specify the
intermediate states (before committing the write buffer or memstate).

src/ConcurrentFS.v
@@ -14,86 +14,54 @@ Import Pred.
 Require Import HomeDirProtocol.
 Require Import RelationClasses.
 
+Record FsParams :=
+  { fsmem: ident;
+    fstree: ident;
+    fshomedirs: ident; }.
+
 Section ConcurrentFS.
 
-  Context {OtherSt:StateTypes}.
-
-  Record FsMem :=
-    fsMem { fsmem: memstate;
-            fs_other_mem: Mem OtherSt; }.
-
-  Record FsAbstraction :=
-    fsAbstraction { fstree: dirtree;
-                    homedirs: TID -> list string;
-                    fs_other_s : Abstraction OtherSt; }.
-
-  Definition St := OptimisticCache.St
-                     {| Mem := FsMem;
-                        Abstraction := FsAbstraction; |}.
-
   Variable fsxp: fs_xparams.
+  Variable CP:CacheParams.
+  Variable P:FsParams.
 
-  Definition get_fsmem (m: Mem St) :=
-    fsmem (cache_other_mem m).
-  Definition get_fstree (sigma: Sigma St) :=
-    fstree (cache_other_s (Sigma.s sigma)).
-  Definition get_homedirs (sigma: Sigma St) :=
-    homedirs (cache_other_s (Sigma.s sigma)).
-
-  Definition fs_invariant wb (sigma: Sigma St) :=
-    let tree := get_fstree sigma in
-    let mscs := get_fsmem (Sigma.mem sigma) in
-    CacheRep wb sigma /\
+  Definition fs_rep vd hm mscs tree :=
     exists ds ilist frees,
       LOG.rep (FSLayout.FSXPLog fsxp) (SB.rep fsxp)
-              (LOG.NoTxn ds) (MSLL mscs) (Sigma.hm sigma)
-              (seq_disk sigma) /\
+              (LOG.NoTxn ds) (MSLL mscs) hm (add_buffers vd) /\
       (DirTreeRep.rep fsxp Pred.emp tree ilist frees)
         (list2nmem (ds!!)).
 
-  Definition fs_guarantee' wb' tid (sigma sigma':Sigma St) :=
-    fs_invariant empty_writebuffer sigma /\
-    fs_invariant wb' sigma' /\
-    let tree := get_fstree sigma in
-    let tree' := get_fstree sigma' in
-    homedir_guarantee tid (get_homedirs sigma) tree tree' /\
-    get_homedirs sigma' = get_homedirs sigma.
+  Definition fs_invariant d hm tree (homedirs: TID -> list string) : heappred :=
+    (fstree P |-> val fstree *
+     fshomedirs P |-> abs homedirs *
+     exists mscs vd, CacheRep CP d empty_writebuffer vd vd *
+                fsmem P |-> val mscs *
+                [[ fs_rep vd hm mscs tree ]])%pred.
 
-  Definition fs_guarantee :=
-    fs_guarantee' empty_writebuffer.
+  Definition fs_guarantee tid (sigma sigma': Sigma) :=
+    exists tree tree' homedirs,
+      fs_invariant (Sigma.disk sigma) (Sigma.hm sigma) tree homedirs (Sigma.mem sigma) /\
+      fs_invariant (Sigma.disk sigma') (Sigma.hm sigma') tree' homedirs (Sigma.mem sigma') /\
+      homedir_guarantee tid homedirs tree tree'.
 
   (* TODO: eventually abstract away protocol *)
-
-  (* TODO: provide mem/abstraction setter/updater in cache, and here: callers
-  should not have to deal with listing out the other parts of these records *)
-
-  Definition set_fsmem (m: Mem St) fsm : Mem St :=
-    let other := fs_other_mem (cache_other_mem m) in
-    cacheMem (St:={|Mem:=FsMem|}) (cache m)
-             (fsMem fsm other).
-
-  Definition upd_fstree update (s: Abstraction St) : Abstraction St :=
-    let fsS0 := cache_other_s s in
-    let other := fs_other_s fsS0 in
-    cacheS (St:={|Abstraction:=FsAbstraction|}) (vdisk_committed s) (vdisk s)
-           (fsAbstraction (update (fstree fsS0)) (homedirs fsS0) other).
 
   Definition guard {T} (r: Result T) : {exists v, r=Success v} + {r=Failed}.
     destruct r; eauto.
   Defined.
 
   Definition retry_syscall T
-             (p: memstate -> @cprog St (Result (memstate * T) * WriteBuffer))
+             (p: memstate -> cprog (Result (memstate * T) * WriteBuffer))
              (update: dirtree -> dirtree)
     : cprog (Result T) :=
-    retry guard (m <- Get;
-                   do '(r, wb) <- p (get_fsmem m);
+    retry guard (ms <- Get _ (fsmem P);
+                   do '(r, wb) <- p ms;
                    match r with
                    | Success (ms', r) =>
-                     _ <- CacheCommit wb;
-                       m <- Get;
-                       _ <- Assgn (set_fsmem m ms');
-                       _ <- GhostUpdate (fun _ s => upd_fstree update s);
+                     _ <- CacheCommit CP wb;
+                       _ <- Assgn (fsmem P) ms';
+                       _ <- GhostUpdate (fstree P) (fun _ => update);
                        Ret (Success r)
                    | Failed =>
                      _ <- CacheAbort;
@@ -101,11 +69,13 @@ Section ConcurrentFS.
                        Ret Failed
                    end).
 
-  Definition file_get_attr inum : @cprog St _ :=
+  Definition file_get_attr inum :=
     retry_syscall (fun mscs =>
-                     OptFS.file_get_attr _ fsxp inum mscs empty_writebuffer)
+                     OptFS.file_get_attr CP fsxp inum mscs empty_writebuffer)
                   (fun tree => tree).
 
+  (* should just be destruct_lift *)
+  (*
   Ltac split_lift_prop :=
     unfold Prog.pair_args_helper in *; simpl in *;
     repeat match goal with
@@ -115,91 +85,70 @@ Section ConcurrentFS.
              apply sep_star_lift_apply in H
            | [ H : _ /\ _ |- _ ] => destruct H
            | _ => progress subst
-           end.
+           end. *)
 
   Section GetAttrCleanSpec.
 
     Hint Extern 0 {{ OptFS.file_get_attr _ _ _ _ _; _ }} => apply OptFS.file_get_attr_ok : prog.
 
-    Ltac descend :=
-      repeat match goal with
-             | [ |- exists _, _ ] => eexists
-             end.
-
-    Lemma fstree_locally_modified : forall sigma sigma',
-        locally_modified sigma sigma' ->
-        get_fstree sigma' = get_fstree sigma.
-    Proof.
-      unfold get_fstree, locally_modified.
-      destruct sigma, sigma'; simpl; intuition congruence.
-    Qed.
+    Ltac break_tuple :=
+      match goal with
+      | [ H: context[let (n, m) := ?a in _] |- _ ] =>
+        let n := fresh n in
+        let m := fresh m in
+        destruct a as [m n]; simpl in H
+      | [ |- context[let (n, m) := ?a in _] ] =>
+        let n := fresh n in
+        let m := fresh m in
+        destruct a as [m n]; simpl
+      end.
 
     Theorem file_get_attr1_ok : forall inum tid mscs,
         cprog_spec fs_guarantee tid
-                   (fun '(pathname, f) '(sigma_i, sigma) =>
+                   (fun '(F, vd0, vd, tree, pathname, f) '(sigma_i, sigma) =>
                       {| precondition :=
-                           fs_guarantee tid sigma_i sigma /\
-                           mscs = get_fsmem (Sigma.mem sigma) /\
-                           let tree := get_fstree sigma in
+                           (F * CacheRep CP (Sigma.disk sigma)
+                                         empty_writebuffer vd0 vd)%pred (Sigma.mem sigma) /\
+                           fs_rep vd (Sigma.hm sigma) mscs tree /\
                            find_subtree pathname tree = Some (TreeFile inum f);
                          postcondition :=
                            fun '(sigma_i', sigma') '(r, wb') =>
-                             get_fstree sigma' = get_fstree sigma /\
-                             match r with
-                             | Success (mscs', (r, _)) =>
-                               r = BFILE.BFAttr f /\
-                               fs_guarantee' wb' tid sigma_i'
-                                             (Sigma.set_mem sigma' (set_fsmem (Sigma.mem sigma') mscs'))
-                             | Failed =>
-                               (* need to promise committed disk doesn't change *)
-                               locally_modified sigma sigma' /\
-                               CacheRep wb' sigma'
-                             end
-                      |}) (OptFS.file_get_attr _ fsxp inum mscs empty_writebuffer).
+                             exists vd',
+                               (F * CacheRep CP (Sigma.disk sigma') wb' vd0 vd')%pred (Sigma.mem sigma') /\
+                               match r with
+                               | Success (mscs', (r, _)) =>
+                                 r = BFILE.BFAttr f /\
+                                 fs_rep vd' (Sigma.hm sigma') mscs' tree
+                               | Failed =>
+                                 fs_rep vd (Sigma.hm sigma') mscs tree
+                               end
+                      |}) (OptFS.file_get_attr CP fsxp inum mscs empty_writebuffer).
     Proof.
       intros.
       step.
 
       unfold OptFS.framed_spec, translate_spec; simpl.
-      repeat apply exists_tuple; simpl.
-      unfold fs_guarantee, fs_guarantee', fs_invariant in *; intuition;
-        repeat deex.
+      repeat apply exists_tuple.
+      repeat break_tuple; simpl in *.
+      unfold fs_rep in *; SepAuto.destruct_lifts; intuition;
+        repeat (deex || SepAuto.destruct_lifts).
 
       descend; intuition eauto.
       SepAuto.pred_apply; SepAuto.cancel; eauto.
 
       step.
+      repeat break_tuple; simpl in *; intuition;
+        repeat deex.
 
-      intuition eauto.
-      apply fstree_locally_modified; auto.
-
-      destruct a.
+      destruct a; simpl in *.
       - (* translated code returned success *)
-        destruct v as (mscs' & (attr & u)); destruct u.
-        split_lift_prop; auto.
-        intuition eauto.
-
-        destruct sigma, sigma'; simpl in *; eauto.
-
-        fold St in *.
-        unfold locally_modified, get_fstree in *.
-        destruct sigma, sigma'; simpl in *; eauto.
-        exists ds, ilist, frees.
-        intuition eauto.
-        congruence.
-
-        unfold locally_modified, get_fstree in *.
-        destruct sigma, sigma' in *; simpl in *; intuition eauto.
-        etransitivity; eauto.
-        match goal with
-        | [ |- homedir_guarantee _ _ ?tree ?tree' ] =>
-          replace tree' with tree by congruence
-        end; reflexivity.
-
-        unfold get_homedirs, set_fsmem, get_fstree, locally_modified in *.
-        destruct sigma_i, sigma, sigma' in *; simpl in *; intuition.
-        congruence.
-      - intuition eauto.
+        repeat break_tuple.
+        unfold Prog.pair_args_helper in *.
+        SepAuto.destruct_lifts; intuition eauto.
+        descend; intuition eauto.
+      - descend; intuition eauto.
+        descend; intuition eauto.
+        eapply LOG.rep_hashmap_subset; eauto.
     Qed.
 
   End GetAttrCleanSpec.
